utp_ap_examples.thy
@@ -6,7 +6,7 @@ text \<open>
 \<close>
 
 theory utp_ap_examples
-  imports utp_ap_rad
+  imports utp_ap_ops
 begin
 
 (* Paper Example 22: Theorem 39 applied to Chaos_RAD = RAD true. *)
@@ -44,5 +44,266 @@ lemma H1_RA1_bottom_AP_example:
     (($rad_wait_lens\<^sup><)\<^sub>e \<and> ades_state_choice))"
   by (simp only: comp_apply RA1_AP_RAD[simplified comp_apply]
       bottom_RAD_is_Chaos H1_Chaos_RAD_example)
+
+(* Paper Example 26 / Thesis Example 44: the angel avoids the
+   divergence of Chaos_AP by resolving the choice in favour of
+   deadlock. *)
+lemma Stop_Skip_seq_Chaos_AP:
+  "(Stop\<^sub>A\<^sub>P \<squnion>\<^sub>A\<^sub>P Skip\<^sub>A\<^sub>P) ;;\<^sub>D\<^sub>A Chaos\<^sub>A\<^sub>P =
+   Stop\<^sub>A\<^sub>P"
+proof -
+  let ?J = "stop_post \<and> skip_post"
+  have J_wf: "(?J \<^sub>f) = ?J"
+    by (simp only: rad_wait_false_conj rad_wait_false_stop_post
+        rad_wait_false_skip_post)
+  have J_PBMH: "PBMH_ades ?J = ?J"
+    by (rule Healthy_if, rule PBMH_ades_conj_closure;
+        simp add: Healthy_def')
+  have J_ok: "?J\<lbrakk>True/ok\<^sup>>\<rbrakk> = ?J"
+    by (simp add: usubst)
+  have choice_AP:
+    "Stop\<^sub>A\<^sub>P \<squnion>\<^sub>A\<^sub>P Skip\<^sub>A\<^sub>P = AP (true \<turnstile> ?J)"
+    apply (simp only: AP_angelic_choice Stop_AP_design Skip_AP_design
+        AP_true_design[OF J_wf J_PBMH J_ok] RA2_conj
+        RA2_stop_post RA2_skip_post RA1_conj)
+    apply (simp add: design_inf expr_if_def fun_eq_iff)
+    by pred_auto
+  \<comment> \<open>A non-waiting handover is impossible: the deadlocked branch
+      has no non-waiting final state.\<close>
+  have handover_false:
+    "(RA1 ?J ;;\<^sub>A\<^sub>D (\<not> rad_wait_lens\<^sup><)) = false"
+    by (simp add: RA1_def aseq_ades_def stop_post_def skip_post_def
+        ades_singleton_choice_def fun_eq_iff Let_def; pred_auto; auto)
+  \<comment> \<open>The angel keeps only the waiting branch, which is deadlock.\<close>
+  have continuation_stop:
+    "(RA1 ?J ;;\<^sub>A\<^sub>D
+      (ades_state_choice \<triangleleft> $rad_wait_lens\<^sup>< \<triangleright> true)) =
+     stop_post"
+    apply (simp add: RA1_def aseq_ades_def stop_post_def
+        skip_post_def ades_singleton_choice_def ades_state_choice_def
+        expr_if_def rad_trace_extensions_def true_pred_def
+        fun_eq_iff Let_def)
+    apply clarify
+    subgoal for a b
+      by (cases "astate.s\<^sub>v (des_vars.more a)";
+          cases "des_vars.more a"; cases a;
+          cases "des_vars.more b"; cases b;
+          auto simp add: lens_defs des_vars.ok_def rad_state.wait_def
+            astate.s_def des_vars.more\<^sub>L_def conj_pred_def
+            true_pred_def intro: order_trans;
+          rule_tac x="rad_state.wait\<^sub>v_update (\<lambda>_. False) y"
+            in bexI;
+          auto)
+    done
+  show ?thesis
+    apply (simp only: choice_AP)
+    by (simp only: AP_true_design_seq_Chaos[OF J_wf J_PBMH J_ok]
+        handover_false continuation_stop pred_ba.compl_bot_eq Stop_AP_def)
+qed
+
+subsection \<open>Prefixing into divergence (Example 27, Lemma 14)\<close>
+
+(* Support laws kept in this session instead of the reactive angelic
+   design layer so the parent session heaps stay valid. *)
+
+(* Trace normalisation fixes the failure observation of the prefixed
+   Chaos: both sides state that the event has occurred. *)
+lemma RA2_prefix_diverge_post:
+  "RA2 (prefix_diverge_post a) = prefix_diverge_post a"
+proof -
+  have append_le:
+    "xs \<le> ys \<Longrightarrow> zs \<le> ys - xs \<Longrightarrow>
+     xs @ zs \<le> ys" for xs ys zs :: "'e list"
+  proof -
+    assume xy: "xs \<le> ys" and zd: "zs \<le> ys - xs"
+    have "xs + zs \<le> xs + (ys - xs)"
+      by (rule add_left_mono[OF zd])
+    also have "... = ys"
+      by (rule diff_add_cancel_left'[OF xy])
+    finally show "xs @ zs \<le> ys"
+      by (simp only: plus_list_def)
+  qed
+  have diff_le:
+    "xs @ zs \<le> ys \<Longrightarrow> zs \<le> ys - xs"
+    for xs ys zs :: "'e list"
+  proof -
+    assume xyz: "xs @ zs \<le> ys"
+    have xy: "xs \<le> ys"
+      by (rule list_append_prefixD[OF xyz])
+    have "xs + zs \<le> xs + (ys - xs)"
+      using xyz diff_add_cancel_left'[OF xy]
+      by (simp only: plus_list_def)
+    then show "zs \<le> ys - xs"
+      by (rule add_le_imp_le_left)
+  qed
+  show ?thesis
+    apply (simp add: RA2_def prefix_diverge_post_def
+        rad_normalise_choices_def rad_trace_difference_def
+        rad_zero_trace_def fun_eq_iff Let_def)
+    apply pred_auto
+    subgoal for ok tr ref wait more morea okv ac moreb refv waitv trv
+      by (frule (1) append_le,
+          rule_tac x="\<lparr>rad_state.tr\<^sub>v = trv, ref\<^sub>v = refv,
+            wait\<^sub>v = waitv\<rparr>" in bexI; simp)
+    subgoal for trv acv trv2 refv waitv
+      by (frule list_append_prefixD, frule diff_le,
+          rule_tac x="trv2 - trv" in exI, rule conjI,
+          rule_tac x=refv in exI, rule_tac x=waitv in exI,
+          rule_tac x=trv2 in exI; simp)
+    done
+qed
+
+lemma RA2_prefix_offer_post:
+  "RA2 (prefix_offer_post a) = prefix_offer_post a"
+proof -
+  \<comment> \<open>List instance of \<open>minus_zero_eq\<close>, shaped for the trace
+      difference the normalisation exposes.\<close>
+  have nil: "xs \<le> ys \<Longrightarrow> ys - xs = [] \<Longrightarrow> ys = xs"
+      for xs ys :: "'e list"
+    using minus_zero_eq by (auto simp add: zero_list_def)
+  show ?thesis
+  apply (simp add: RA2_def prefix_offer_post_def
+      rad_normalise_choices_def rad_trace_difference_def
+      rad_zero_trace_def fun_eq_iff Let_def)
+  apply pred_auto
+  subgoal for ok tr ref wait more morea okv ac moreb refv waitv trv
+    by (drule sym, frule (1) nil,
+        rule_tac x="\<lparr>rad_state.tr\<^sub>v = trv, ref\<^sub>v = refv,
+          wait\<^sub>v = True\<rparr>" in bexI; simp)
+  subgoal for tr ac ref wait
+    by (rule_tac x=ref in exI, rule_tac x=True in exI, rule conjI,
+        rule_tac x=tr in exI,
+        simp_all add: diff_cancel zero_list_def)
+  done
+qed
+
+(* The ok-in counterpart of RA1_unrest_ok_out, for the RA1-true
+   failure condition of ChaosCSP_AP. *)
+lemma RA1_unrest_ok_in [unrest]:
+  "$ok\<^sup>< \<sharp> P \<Longrightarrow> $ok\<^sup>< \<sharp> RA1 P"
+  apply (simp add: unrest_lens RA1_def Let_def)
+  apply (simp add: subst_app_def subst_upd_def subst_id_def
+      SEXP_def lens_defs alpha_defs)
+  done
+
+(* Handing the prefix over to any non-waiting continuation is always
+   possible: performing the event reaches a non-waiting state. *)
+lemma prefix_handover_nonwait:
+  "(RA1 (prefix_post a) ;;\<^sub>A\<^sub>D (\<not> rad_wait_lens\<^sup><)) = true"
+  apply (simp add: RA1_def aseq_ades_def prefix_post_def
+      ades_singleton_choice_def expr_if_def
+      rad_state.wait_def rad_trace_extensions_def fun_eq_iff
+      Let_def lens_defs rad_state.wait_def astate.s_def
+      des_vars.more\<^sub>L_def true_pred_def conj_pred_def
+      not_pred_def SEXP_def subst_ext_def
+      subst_app_def ex_in_conv[symmetric])
+  apply (rule allI, rule conjI)
+  subgoal for aa
+    by (rule_tac x="\<lparr>rad_state.tr\<^sub>v =
+        rad_state.tr\<^sub>v (astate.s\<^sub>v (des_vars.more aa)) @ [a],
+        ref\<^sub>v = {}, wait\<^sub>v = False\<rparr>" in bexI;
+        simp add: trace_le_append)
+  subgoal for aa
+    by (rule_tac x="\<lparr>rad_state.tr\<^sub>v =
+        rad_state.tr\<^sub>v (astate.s\<^sub>v (des_vars.more aa)) @ [a],
+        ref\<^sub>v = {}, wait\<^sub>v = False\<rparr>" in exI;
+        simp add: trace_le_append)
+  done
+
+(* Paper Example 27 / Thesis Example 45: the potential for divergence
+   after the event leads to immediate divergence. *)
+lemma Prefix_Chaos_AP:
+  "(a \<rightarrow>\<^sub>A\<^sub>P Chaos\<^sub>A\<^sub>P) = Chaos\<^sub>A\<^sub>P"
+  unfolding Prefix_AP_def PrefixSkip_AP_def
+  apply (subst AP_true_design_seq_Chaos[OF PrefixSkip_AP_facts])
+  by (simp only: prefix_handover_nonwait pred_ba.compl_top_eq
+      design_false_pre Chaos_AP_def)
+
+(* Thesis Section 6.4.8: the compound a \<rightarrow>\<^sub>A\<^sub>P Skip\<^sub>A\<^sub>P
+   coincides with the Definition 57 primitive, as at the RAD layer
+   (Prefix_Skip_RAD_RA). *)
+lemma Prefix_Skip_AP:
+  "(a \<rightarrow>\<^sub>A\<^sub>P Skip\<^sub>A\<^sub>P) = PrefixSkip_AP a"
+  unfolding Prefix_AP_def PrefixSkip_AP_def Skip_AP_def
+  apply (subst AP_true_design_seq[OF PrefixSkip_AP_facts Skip_AP_facts])
+  by (simp only: prefix_continuation_skip)
+
+(* Paper Lemma 14 / Thesis Lemma L.6.4.6: prefixing into ChaosCSP_AP
+   cannot backtrack the event to avoid the divergence that follows,
+   mirroring a \<rightarrow>\<^sub>R\<^sub>A\<^sub>D Chaos\<^sub>R\<^sub>A\<^sub>D
+   (Prefix_Chaos_RAD_RA). *)
+lemma Prefix_ChaosCSP_AP:
+  "(a \<rightarrow>\<^sub>A\<^sub>P ChaosCSP\<^sub>A\<^sub>P) =
+   AP ((\<not> prefix_diverge_post a) \<turnstile> prefix_offer_post a)"
+proof -
+  let ?pdp = "prefix_diverge_post a"
+  let ?pop = "prefix_offer_post a"
+  have prefix_PBMH: "RA1 (prefix_post a) is PBMH_ades"
+    by (rule RA1_PBMH_ades_closure) (simp add: Healthy_def')
+  have prefix_shape:
+    "PrefixSkip_AP a =
+     ((true \<triangleleft> $rad_wait_lens\<^sup>< \<triangleright> (\<not> false)) \<turnstile>
+      (ades_state_choice \<triangleleft> $rad_wait_lens\<^sup>< \<triangleright>
+       RA1 (prefix_post a)))"
+    by (simp only: PrefixSkip_AP_design pred_ba.compl_bot_eq
+        expr_if_idem)
+  have chaoscsp_shape:
+    "(ChaosCSP\<^sub>A\<^sub>P :: ('e list, 'e) reactive_angelic_design) =
+     ((true \<triangleleft> $rad_wait_lens\<^sup>< \<triangleright> (\<not> RA1 true)) \<turnstile>
+      (ades_state_choice \<triangleleft> $rad_wait_lens\<^sup>< \<triangleright> false))"
+    apply (simp only: ChaosCSP_AP_design)
+    by (simp add: expr_if_def fun_eq_iff; pred_auto)
+  have seq_form:
+    "(a \<rightarrow>\<^sub>A\<^sub>P ChaosCSP\<^sub>A\<^sub>P) =
+     RA3AP ((\<not> ?pdp) \<turnstile> (?pop \<or> ?pdp))"
+    unfolding Prefix_AP_def
+    apply (subst prefix_shape, subst chaoscsp_shape)
+    apply (subst AP_wait_design_seq[
+        where F=false and T="RA1 (prefix_post a)"
+          and G="RA1 true" and U=false])
+          apply (simp_all add: unrest false_PBMH_ades prefix_PBMH)
+    by (simp only: aseq_ades_false_left pred_ba.compl_bot_eq
+        pred_ba.inf_top_left pred_impl_laws pred_ba.double_compl
+        prefix_handover_diverge[unfolded RA2_RA1_true]
+        prefix_continuation_chaos[unfolded RA2_RA1_true])
+  have design_eq:
+    "((\<not> ?pdp) \<turnstile> ?pop) =
+     ((\<not> ?pdp) \<turnstile> (?pop \<or> ?pdp))"
+    by pred_auto
+  have N_PBMH:
+    "((\<not> ?pdp) \<turnstile> (?pop \<or> ?pdp)) is PBMH_ades"
+    by (rule PBMH_ades_design_closure;
+        simp add: Healthy_def' PBMH_ades_disj)
+  have absorb:
+    "(ac_non_empty \<and> ((\<not> ?pdp) \<and> (?pop \<or> ?pdp))) =
+     ((\<not> ?pdp) \<and> (?pop \<or> ?pdp))"
+    by pred_auto
+  have RA2_N:
+    "RA2 ((\<not> ?pdp) \<turnstile> (?pop \<or> ?pdp)) =
+     ((\<not> ?pdp) \<turnstile> (?pop \<or> ?pdp))"
+    by (simp only: RA2_design_distrib RA2_not RA2_disj
+        RA2_prefix_diverge_post RA2_prefix_offer_post)
+  have recognised:
+    "AP ((\<not> ?pdp) \<turnstile> (?pop \<or> ?pdp)) =
+     RA3AP ((\<not> ?pdp) \<turnstile> (?pop \<or> ?pdp))"
+    apply (subst AP_design_RA3AP_RA2[
+        OF _ _ N_PBMH RA1_true_absorb_lift[OF absorb]])
+    by (simp_all add: unrest RA2_N)
+  show ?thesis
+    by (simp only: seq_form design_eq recognised)
+qed
+
+subsection \<open>Avoiding divergence altogether (Example 28)\<close>
+
+(* Paper Example 28 / Thesis Example 46: the angel avoids the
+   divergence following the event a altogether by choosing the
+   prefixing on b, a property not available in the theory of
+   reactive angelic designs (Prefix_Skip_Chaos_different_events). *)
+lemma Prefix_Chaos_Skip_angelic_choice:
+  "(a \<rightarrow>\<^sub>A\<^sub>P Chaos\<^sub>A\<^sub>P) \<squnion>\<^sub>A\<^sub>P (b \<rightarrow>\<^sub>A\<^sub>P Skip\<^sub>A\<^sub>P) = (b \<rightarrow>\<^sub>A\<^sub>P Skip\<^sub>A\<^sub>P)"
+  apply (simp only: Prefix_Chaos_AP)
+  apply (subst inf.commute)
+  by (rule Chaos_AP_angelic_choice_unit[
+        OF Prefix_AP_closure[OF Skip_AP_is_AP]])
 
 end
